Runtime/Network/Execution/Propagate.lean
@@ -6,30 +6,32 @@ def Sib (reactor : ReactorId net) := { id : ReactorId net // id ≂ reactor }
 
 -- Note: By the definition of `Connections`, the root reactor can't have a connection to itself.
 --       Hence, if `reactor` = `sib` = `nil`, we automatically get `none`. 
-private def aux (exec : Executable net) {reactor : ReactorId net} (sib : Sib reactor) (dst : sib.val.inputs.vars) : Option (sib.val.inputs.type dst) :=
+private def aux (exec : Executable net) (reaction : ReactionId net) (sib : Sib reaction.reactor) (dst : sib.val.inputs.vars) : Option (sib.val.inputs.type dst) :=
   if h₁ : sib.val.isRoot then 
     none -- cf. note above
   else
-    let parent := sib.val.prefix (Graph.Path.isCons_iff_not_isNil.mpr h₁)
-    let subport : Graph.Class.Subport parent.class .input := sorry -- ⟨sorry, dst⟩  -- CONTINUE HERE
-    match h₂ : parent.class.connections.source subport with
+    let split := sib.val.split (Graph.Path.isCons_iff_not_isNil.mpr h₁) -- TODO: We can't destruct here because then the type cast on `dst` doesn't work.
+    let parent := split.fst
+    let leaf := split.snd
+    match h₂ : parent.class.connections.source ⟨leaf, Graph.Path.split_class (path := sib.val) ▸ dst⟩ with
     | none => none -- independent
     | some src => 
-      if h₃ : src.child.class = reactor.class then 
-        have H := parent.class.connections.eqType h₂             -- (subport.child.class.interface .inputs).type subport.port = (src.child.class.interface .outputs).type src.port
-        let a := exec.interface reactor .outputs (h₃ ▸ src.port) -- Option (reactor.class.interface .outputs).type (h₃ ▸ src.port)
-        sorry                                                    -- Option (sib.val.inputs.type dst)
+      -- TODO: Make this check more precise, by checking whether the given port is an effect of the reaction.
+      if h₃ : src.child.class = reaction.reactor.class then 
+        have H := parent.class.connections.eqType h₂                      -- (subport.child.class.interface .inputs).type subport.port = (src.child.class.interface .outputs).type src.port
+        let a := exec.interface reaction.reactor .outputs (h₃ ▸ src.port) -- Option (reactor.class.interface .outputs).type (h₃ ▸ src.port)
+        sorry                                                             -- Option (sib.val.inputs.type dst)
       else 
         none -- independent
 
-def propagate (exec : Executable net) (reactor : ReactorId net) : Executable net := { exec with
+def propagate (exec : Executable net) (reaction : ReactionId net) : Executable net := { exec with
   reactors := fun id => { exec.reactors id with
-    interface := if h : id ≂ reactor then sibling exec ⟨id, h⟩ else exec.interface id
+    interface := if h : id ≂ reaction.reactor then sibling exec reaction ⟨id, h⟩ else exec.interface id
   }
 }
 where
-  sibling (exec : Executable net) {reactor : ReactorId net} (sib : Sib reactor) : (kind : Reactor.InterfaceKind) → kind.interfaceType (sib.val.class.interface kind)
-    | .inputs => fun port => (aux exec sib port).orElse (fun _ => exec.interface sib.val .inputs port)
-    | _ => (exec.reactors sib.val).interface _
+  sibling (exec : Executable net) (reaction : ReactionId net) (sib : Sib reaction.reactor) : (kind : Reactor.InterfaceKind) → kind.interfaceType (sib.val.class.interface kind)
+    | .inputs => fun port => (aux exec reaction sib port).orElse (fun _ => exec.interface sib.val .inputs port)
+    | _       => (exec.reactors sib.val).interface _
 
 end Network.Executable
